\documentclass[11pt]{article}
\usepackage{graphics}
\usepackage{amsthm}
\usepackage{amsmath}
\usepackage{amssymb}
\usepackage{listings}
\usepackage{mathtools}
\usepackage[margin=1in]{geometry}

\newenvironment{solution}
  {\renewcommand\qedsymbol{$\blacksquare$}\begin{proof}[Solution]}
  {\end{proof}}
  
\newcommand{\N}{\mathbb{N}}
\setlength\parindent{0pt}
\begin{document}

	\hrule
	\begin{center}
		{\Large Homework 3} \\ % Replace with the homework number
		\vspace{0.2cm}
		Partial Differential Equations, Spring 2023 \hfill David Yang % Replace with your name(s)
	\end{center}

\hrule

\vspace{1em}

\underline{Logan Chapter 1.5, Problem 5} \\

\textbf{The total energy of the string governed by equation (1.37) with boundary conditions (1.40) is defined by $$E(t) = \int_{0}^{\ell} \left( \frac{1}{2} \rho_0 u_t^2 + \frac{1}{2} \tau_0 u_x^2 \right) \, dx.$$}

\textbf{Show that the total energy is constant for all $ t \geq 0$. Hint: Multiply (1.37) by $u_t$ and note that $(u_t^2)_t = 2u_tu_{tt}$ and $(u_tu_x)_x = u_tu_{xx} + u_{tx}u_x.$ Then
show that $$\frac{d}{dt} \int_{0}^{\ell} \rho_0 u_t^2 \, dx= [2\tau_0u_tu_x]_0^\ell - \frac{d}{dt}  \int_{0}^{\ell} \tau_0 u_x^2 \, dx.$$ }

\begin{solution} 
We follow the hint provided in the book. We begin with equation (1.37): $$ \rho_0 (x) u_{tt} = \tau_0 u_{xx}.$$

Multiplying both sides by $u_t$, we get that $$ \rho_0 (x) u_t u_{tt} = \tau_0 u_t u_{xx}.$$

Since $(u_t^2)_t = 2u_tu_{tt}$ and $(u_tu_x)_x = u_tu_{xx} + u_{tx} u_x,$ we have that $$u_tu_{tt} = \frac{1}{2}\left(u_t^2\right)_t \text { and } u_tu_{xx} = (u_tu_x)_x - u_{tx}u_x.$$

Substituting these results into the equation $ \rho_0 (x) u_t u_{tt} = \tau_0 u_t u_{xx}$, we find that

$$ \frac{1}{2} \left(u_t^2\right)_t \rho_0 = \tau_0 \left( (u_tu_x)_x - u_{tx}u_x\right).$$

Integrating both sides of the equation with respect to $x$ and bounding the integral at $x=0$ and $x = \ell$, we get that

$$ \int_0^{\ell} \frac{1}{2} \left(u_t^2\right)_t \rho_0 \, dx = \tau_0 \int_0^{\ell} (u_tu_x)_x - u_{tx} u_x \, dx.$$


Splitting the integral on the right-hand side into two separate integrals and simplifying, we get that

$$ \int_0^{\ell} \frac{1}{2} \left(u_t^2\right)_t \rho_0 \, dx = [\tau_0u_tu_x]_0^{\ell} - \int_0^{\ell} \tau_0u_{tx} u_x \, dx.$$

We can simplify further -- note that we can move $\frac{d}{dt}$ out of the left integral and that $$\int_0^{\ell} \tau_0u_{tx} u_x \, dx = \frac{1}{2} \frac{d}{dt} \int_0^{\ell} \tau_0 u_x^2.$$

Substituting these results into the above equation, we get
$$ \frac{d}{dt} \int_0^{\ell} \frac{1}{2} u_t^2 \rho_0 \, dx = [\tau_0u_tu_x]_0^{\ell} - \frac{1}{2} \frac{d}{dt} \int_0^{\ell} \tau_0u_x^2 \, dx.$$

Thus, multiplying both sides by two gives us the desired result:
$$\frac{d}{dt} \int_{0}^{\ell} \rho_0 u_t^2 \, dx= [2\tau_0u_tu_x]_0^\ell - \frac{d}{dt}  \int_{0}^{\ell} \tau_0 u_x^2 \, dx.$$ 

Going back to the original question, we have that $$E(t) = \int_{0}^{\ell} \left( \frac{1}{2} \rho_0 u_t^2 + \frac{1}{2} \tau_0 u_x^2 \right) \, dx.$$

Thus, taking the derivative of both sides, plugging in our above results, and applying the boundary conditions from Equation 1.40 (since $u(0, t) = u(l, t) = 0$, we also have $u_t(0, t) = u_t(l, t) = 0$), we get that
$$E'(t) =  \frac{1}{2} \frac{d}{dt} \int_0^{\ell} u_t^2 \rho_0 \, dx + \frac{1}{2} \frac{d}{dt} \int_0^{\ell} \tau_0u_x^2 \, dx = [\tau_0u_tu_x]_0^{\ell} = 0. $$

Thus, the total energy $E(t)$ is constant for all $t \geq 0.$
\end{solution}
\end{document}